---
title: "EX2"
author: "roi hezkiyahu"
date: "4 3 2022"
output: html_document
---

```{r setup, include=FALSE}
knitr::opts_chunk$set(echo = TRUE)
```

![Q1](Q1.png)

**a**

$$
Reminder\, of \, assumtions:
\\(1) \sum_{i=1}^I\alpha_i = 0
\\(2) \sum_{j=1}^I\beta_j = 0
\\(3) \sum_{i=1}^I\gamma_{ij} = 0\,\,\, \forall j
\\(4) \sum_{j=1}^I\gamma_{ij} = 0\,\,\, \forall i
\\\mu_{.j} -\mu = \frac{1}{nI}\sum_{i=1}^I\sum_{k=1}^n(\mu_{ij}) - \mu = \frac{1}{nI}\sum_{i=1}^I\sum_{k=1}^n(\mu +\alpha_i +\beta_j +\gamma_{ij}) - \mu = \frac{1}{nI}nI\mu + \frac{n\sum_{i=1}^I\alpha_i}{nI} + \frac{nI\beta_j}{nI} + \frac{n\sum_{i=1}^I\gamma_{ij}}{nI} - \mu =\\
=\mu + \frac{\sum_{i=1}^I\alpha_i}{I} + \beta_j + \frac{\sum_{i=1}^I\gamma_{ij}}{I} - \mu := A + \beta_j + C
\\
\\ (1),(3) \Rightarrow A=C=0 \Rightarrow \mu_{.j} -\mu = \beta_j
$$

**b**

$$
\gamma_{ij} = \mu_{ij} - \mu - \alpha_i -  \beta_j = \mu_{ij} - \mu -(\mu_{.j} -\mu) - (\mu_{i.} -\mu) = \mu_{ij} +2\mu - \mu -\mu_{i.} -  \mu_{.j} = \mu_{ij} -\mu_{i.} -  \mu_{.j} + \mu
$$

**c**

$$
MSA = \frac{SSA}{I-1} = \frac{nJ\sum_{i=1}^I(\bar Y_{i..} - \bar Y)^2}{I-1}
\\\bar Y_{i..} - \bar Y = \frac{1}{nJ}\sum_{j=1}^J\sum_{k=1}^nY_{ijk} - \frac{1}{N}\sum_{i=1}^I\sum_{j=1}^J\sum_{k=1}^nY_{ijk}=\frac{1}{nJ}\sum_{j=1}^J\sum_{k=1}^n(\mu + \alpha_i+\beta_j+\gamma_{ij}+\varepsilon_{ijk}) - \frac{1}{N}\sum_{i=1}^I\sum_{j=1}^J\sum_{k=1}^n(\mu + \alpha_i+\beta_j+\gamma_{ij}+\varepsilon_{ijk})=\\
=\mu +\alpha_i+0+0+\bar \varepsilon_{i..} - (\mu +0 +0 +0 +\bar \varepsilon) = \alpha_i - (\bar \varepsilon + \bar \varepsilon_{i..})\Rightarrow (\bar Y_{i..} - \bar Y)^2 = \alpha_i^2 +2\alpha_i(\bar\varepsilon_{i..} - \bar \varepsilon) + (\bar\varepsilon_{i..} - \bar \varepsilon)^2
\\E(MSA) = E(\frac{nJ\sum_{i=1}^I(\alpha_i^2 +2\alpha_i(\bar\varepsilon_{i..} - \bar \varepsilon) + (\bar\varepsilon_{i..} - \bar \varepsilon)^2)}{I-1}) = \frac{nJ\sum_{i=1}^I\alpha_i^2}{I-1} + \frac{2nJ\sum_{i=1}\alpha_i E(\bar\varepsilon_{i..} - \bar \varepsilon)}{I-1} + \frac{E(nJ\sum_{i=1}^I(\bar\varepsilon_{i..} - \bar \varepsilon)^2)}{I-1}\\
(5) \frac{2nJ\sum_{i=1}^I\alpha_i E(\bar\varepsilon_{i..} - \bar \varepsilon)}{I-1} = \frac{nJ\sum_{i=1}^I\alpha_i (-E(\bar \varepsilon) + E(\bar\varepsilon_{i..}))}{I-1} = 0
\\(6) nJ\sum_{i=1}^I\frac{E((\bar\varepsilon_{i..} - \bar \varepsilon)^2)}{I-1} = nJ\sum_{i=1}^I\frac{V(\bar\varepsilon_{i..} - nJ\sum_{i=1}^I\bar \varepsilon)}{I-1} + nJ\sum_{i=1}^I\frac{(E(\bar\varepsilon_{i..} - \bar \varepsilon))^2}{I-1} = nJ\sum_{i=1}^I\frac{V(\bar\varepsilon_{i..} - \bar \varepsilon)}{I-1} = \\
=\frac{nJ}{I-1}\sum_{i=1}^I (\frac{\sigma^2}{nJ}-\frac{\sigma^2}{N}) = \frac{nJ}{I-1} \frac{(I-1)\sigma^2}{nJ} = \sigma^2
\\ E(MSA) =  \frac{nJ\sum_{i=1}^I\alpha_i^2}{I-1} + (5) + (6) = \frac{nJ\sum_{i=1}^I\alpha_i^2}{I-1} + \sigma^2
$$

**d**

$$
(7)\,\bar Y = \frac{1}{N}\sum_{i=1}^I\sum_{j=1}^J\sum_{k=1}^nY_{ijk} = \frac{1}{N}\sum_{i=1}^I\sum_{j=1}^J\sum_{k=1}^n \mu + \alpha_i+\beta_j+\gamma_{ij}+\varepsilon_{ijk} = \mu + \bar \varepsilon
\\(8)\,\bar Y_{i..} = \frac{1}{nJ}\sum_{j=1}^J\sum_{k=1}^nY_{ijk} = \frac{1}{nJ}\sum_{j=1}^J\sum_{k=1}^n \mu + \alpha_i+\beta_j+\gamma_{ij}+\varepsilon_{ijk} = \mu + \alpha_i + \bar \varepsilon_{i..}
\\(9)\,\bar Y_{.j.} = \frac{1}{nI}\sum_{i=1}^I\sum_{k=1}^nY_{ijk} = \frac{1}{nI}\sum_{i=1}^I\sum_{k=1}^n \mu + \alpha_i+\beta_j+\gamma_{ij}+\varepsilon_{ijk} = \mu + \beta_j + \bar \varepsilon_{.j.}
\\(10)\,\bar Y_{ij.} = \frac{1}{n}\sum_{k=1}^nY_{ijk} = \frac{1}{n}\sum_{k=1}^n \mu + \alpha_i+\beta_j+\gamma_{ij}+\varepsilon_{ijk} = \mu + \alpha_i + \beta_j + \gamma_{ij} + \bar \varepsilon_{ij.}
\\(11)\,\bar Y_{i..} - \bar Y = \mu + \alpha_i + \bar \varepsilon_{i..} - \mu - \bar \varepsilon = \alpha_i +\bar \varepsilon_{i..} - \bar \varepsilon
\\(12)\,\bar Y_{ij.}-\bar Y_{i..}-\bar Y_{.j.}+\bar Y =\gamma_{ij}
\\(13)\, \sum_{i=1}^I\sum_{j=1}^J(\bar Y_{i..} - \bar Y)(\bar Y_{ij.}-\bar Y_{i..}-\bar Y_{.j.}+\bar Y) = \sum_{i=1}^I\sum_{j=1}^J(11)(12) = \sum_{i=1}^I\sum_{j=1}^J\gamma_{ij}(\alpha_i +\bar \varepsilon_{i..} - \bar \varepsilon) = \sum_{i=1}^I(0(\alpha_i +\bar \varepsilon_{i..} - \bar \varepsilon)) = 0
$$

![](Q2_1.png)
![Q2](Q2_2.png)